Tenglamani yeching \(\left( x^{2} - 4x + 6 \right)^{2} - 4\left( x^{2} - 4x + 6 \right) + 6 = x\).
Tenglamani yeching \(\left( x^{2} + 10x + 10 \right)\left( x^{2} + x + 10 \right) = 10x^{2}\) .
Tenglamani yeching \(\left( x^{2} - 6x \right)^{2} - 2(x - 3)^{2} = 81\).
Tenglamani yeching \((x + 1)^{5} + (x - 1)^{5} = 32x\).
Tenglamani yeching. \(\sqrt{x + 8 + 2\sqrt{x + 7}} + \sqrt{x + 1 - \sqrt{x + 7}} = 4\).
Tenglamani yeching \(\sqrt{\frac{18 - 7x - x^{2}}{8 - 6x + x^{2}}} + \sqrt{\frac{8 - 6x + x^{2}}{18 - 7x - x^{2}}} = \frac{13}{6}\).
Tenglamani yeching \((x + 4)(x + 1) - 3\sqrt{x^{2} + 5x + 2} = 6\).
Tenglamani yeching. \(\sqrt{x^{2} + x + 4} + \sqrt{x^{2} + x + 1} = \sqrt{2x^{2} + 2x + 9}\).
Tenglamani yeching. \(\sqrt{3x^{2} - 2x + 15} + \sqrt{3x^{2} - 2x + 8} = 7\).
Tenglamani yeching. \(\sqrt{x} + \frac{2x + 1}{x + 2} = 2\).
Tenglamani yeching. \(\frac{4x}{x^{2} + x + 3} + \frac{5x}{x^{2} - 5x + 3} = - \frac{3}{2}\).
Tenglamani yeching. \(\sqrt[3]{x} + \sqrt[3]{x - 16} = \sqrt[3]{x - 8}\).
Tenglamani yeching. \((x - 4)^{3} + (x - 4)^{2} + (x - 4)(x - 3) + (x - 3)^{2} + (x - 3)^{3} = 6\).
Tenglamani yeching. \(\frac{z}{z + 1} - 2\sqrt{\frac{z + 1}{2}} = 3\).
Tenglamani yeching. \(\sqrt[3]{x - 1} + \sqrt[3]{x - 2} - \sqrt{2x - 3} = 0\).
Tenglamani yeching. \((\sqrt{x + 1} + \sqrt{x})^{3} + (\sqrt{x + 1} + \sqrt{x})^{2} = 2\).
Tengsizlikni yeching: \(\sqrt{x^{2} - 4x} > x - 3\).
Tengsizlikni yeching:\(x^{2}\left( x^{4} + 36 \right) - 6\sqrt{3}\left( x^{4} + 4 \right) < 0\).
Tengsizlikni yeching: \(\frac{x^{3} + 3x^{2} - x - 3}{x^{2} + 3x - 10} < 0\).
Tengsizlikni yeching: \(\sqrt{x + 3} + \sqrt{x - 2} - \sqrt{2x + 4} > 0\).